src/Utilities/FisherYates/Correctness.dfy
@@ -8,12 +8,18 @@ module FisherYates.Correctness {
   import Permutations
   import Rand
 
-  lemma {:axiom} CorrectnessFisherYates<T>(xs: seq<T>, p: seq<T>)
+  lemma {:axiom} CorrectnessFisherYatesOne<T>(xs: seq<T>, s: Rand.Bitstream)
+    ensures 
+      var r := Model.Shuffle(xs)(s);
+      && r.Result?
+      && Permutations.IsPermutationOf(xs, r.value)
+
+  lemma {:axiom} CorrectnessFisherTwo<T>(xs: seq<T>, p: seq<T>)
     requires Permutations.IsPermutationOf(p, xs)
-    ensures |Permutations.CalculateAllPermutationsOf(xs)| > 0
     ensures
       var e := iset s | Model.Shuffle(xs)(s).Equals(p);
       && e in Rand.eventSpace
+      && |Permutations.CalculateAllPermutationsOf(xs)| > 0
       && Rand.prob(e) == 1.0 / (|Permutations.CalculateAllPermutationsOf(xs)| as real)
 
 }
